Fstar/Typedefs.fst
@@ -1,0 +1,21 @@
+module Typedefs
+open FStar.Mul
+
+let rec len l = match l with [] -> 0 | _::t -> 1 + len t
+type myList 'a = 
+    | Nil : myList 'a
+    | App : hd: 'a -> tl : myList 'a -> myList 'a
+
+let hd (l: myList 'a{App? l}) : Tot ('a) = match l with 
+    | App h _ -> h 
+let tl (l: myList 'a{App? l}) : Tot (myList 'a) = match l with
+    | App _ t -> t
+
+//_________________________________________________________________________________
+
+let rec get_nth (l:list 'a{Cons? l}) (n:int{ n>=0 && n < (len l)})
+    : Tot 'a (decreases l)
+    = match l with 
+    | h::t ->   if n = 0 then h 
+                else get_nth t (n-1)
+                
